theories/SpecNotations.v
@@ -2,8 +2,9 @@ Require Import Blech.Spec.
 
 Infix "*" := t_prod.
 
-Notation "Γ ⊢ E ? t" := (JE Γ E t) (at level 90).
-Notation "Γ ⊢ v 'in' t" := (Jv Γ v t) (at level 90).
+Infix "⊢" := d_with (at level 30).
+
+Notation "d 'in' t" := (Jv d t) (at level 90).
 
 Notation "v ⇓ N" := (big v N) (at level 90).
 
